Superposition_Calculus/Ground_Type_System.thy
@@ -2,64 +2,64 @@ theory Ground_Type_System
   imports Ground_Clause
 begin
 
-inductive has_type for \<F> where
-  GFun: "
-    \<F> f = (\<tau>s, \<tau>) \<Longrightarrow> list_all2 (has_type \<F>) ts \<tau>s \<Longrightarrow>
-    has_type \<F> (GFun f ts) \<tau>"
+inductive welltyped for \<F> where
+  GFun: "\<F> f = (\<tau>s, \<tau>) \<Longrightarrow> list_all2 (welltyped \<F>) ts \<tau>s \<Longrightarrow> welltyped \<F> (GFun f ts) \<tau>"
 
-lemma right_unique_has_type: "right_unique (has_type \<F>)"
+lemma welltyped_right_unique: "right_unique (welltyped \<F>)"
 proof (rule right_uniqueI)
   fix t \<tau>\<^sub>1 \<tau>\<^sub>2
-  assume "has_type \<F> t \<tau>\<^sub>1" and "has_type \<F> t \<tau>\<^sub>2"
+  assume "welltyped \<F> t \<tau>\<^sub>1" and "welltyped \<F> t \<tau>\<^sub>2"
   thus "\<tau>\<^sub>1 = \<tau>\<^sub>2"
-    by (auto elim!: has_type.cases)
+    by (auto elim!: welltyped.cases)
 qed
 
-definition well_typed_atm where
-  "well_typed_atm \<F> A \<longleftrightarrow> (\<exists>\<tau>. \<forall>t \<in> set_uprod A. has_type \<F> t \<tau>)"
+definition welltyped\<^sub>a where
+  "welltyped\<^sub>a \<F> A \<longleftrightarrow> (\<exists>\<tau>. \<forall>t \<in> set_uprod A. welltyped \<F> t \<tau>)"
 
-definition well_typed_lit where
-  "well_typed_lit \<F> L \<longleftrightarrow> well_typed_atm \<F> (atm_of L)"
+definition welltyped\<^sub>l where
+  "welltyped\<^sub>l \<F> L \<longleftrightarrow> welltyped\<^sub>a \<F> (atm_of L)"
 
-definition well_typed_cls where
-  "well_typed_cls \<F> C \<longleftrightarrow> (\<forall>L \<in># C. well_typed_lit \<F> L)"
+definition welltyped\<^sub>c where
+  "welltyped\<^sub>c \<F> C \<longleftrightarrow> (\<forall>L \<in># C. welltyped\<^sub>l \<F> L)"
 
-definition well_typed_cls_set where
-  "well_typed_cls_set \<F> N \<longleftrightarrow> (\<forall>C \<in> N. well_typed_cls \<F> C)"
+definition welltyped\<^sub>c\<^sub>s where
+  "welltyped\<^sub>c\<^sub>s \<F> N \<longleftrightarrow> (\<forall>C \<in> N. welltyped\<^sub>c \<F> C)"
 
-lemma well_typed_cls_add_mset: "well_typed_cls \<F> (add_mset L C) \<longleftrightarrow> well_typed_lit \<F> L \<and> well_typed_cls \<F> C"
-  by (simp add: well_typed_cls_def)
+lemma welltyped\<^sub>c_add_mset: 
+  "welltyped\<^sub>c \<F> (add_mset L C) \<longleftrightarrow> welltyped\<^sub>l \<F> L \<and> welltyped\<^sub>c \<F> C"
+  by (simp add: welltyped\<^sub>c_def)
 
-lemma well_typed_cls_plus: "well_typed_cls \<F> (C + D) \<longleftrightarrow> well_typed_cls \<F> C \<and> well_typed_cls \<F> D"
-  by (auto simp: well_typed_cls_def)
+lemma welltyped\<^sub>c_plus: 
+  "welltyped\<^sub>c \<F> (C + D) \<longleftrightarrow> welltyped\<^sub>c \<F> C \<and> welltyped\<^sub>c \<F> D"
+  by (auto simp: welltyped\<^sub>c_def)
 
 lemma gctxt_apply_term_preserves_typing:
   assumes
-    \<kappa>_type: "has_type \<F> \<kappa>\<langle>t\<rangle>\<^sub>G \<tau>\<^sub>1" and
-    t_type: "has_type \<F> t \<tau>\<^sub>2" and
-    t'_type: "has_type \<F> t' \<tau>\<^sub>2"
-  shows "has_type \<F> \<kappa>\<langle>t'\<rangle>\<^sub>G \<tau>\<^sub>1"
+    \<kappa>_type: "welltyped \<F> \<kappa>\<langle>t\<rangle>\<^sub>G \<tau>\<^sub>1" and
+    t_type: "welltyped \<F> t \<tau>\<^sub>2" and
+    t'_type: "welltyped \<F> t' \<tau>\<^sub>2"
+  shows "welltyped \<F> \<kappa>\<langle>t'\<rangle>\<^sub>G \<tau>\<^sub>1"
   using \<kappa>_type
 proof (induction \<kappa> arbitrary: \<tau>\<^sub>1)
   case GHole
   then show ?case
     using t_type t'_type
-    using right_unique_has_type[of \<F>, THEN right_uniqueD]
+    using welltyped_right_unique[of \<F>, THEN right_uniqueD]
     by auto
 next
   case (GMore f ss1 \<kappa> ss2)
-  have "has_type \<F> (GFun f (ss1 @ \<kappa>\<langle>t\<rangle>\<^sub>G # ss2)) \<tau>\<^sub>1"
+  have "welltyped \<F> (GFun f (ss1 @ \<kappa>\<langle>t\<rangle>\<^sub>G # ss2)) \<tau>\<^sub>1"
     using GMore.prems by simp
-  hence "has_type \<F> (GFun f (ss1 @ \<kappa>\<langle>t'\<rangle>\<^sub>G # ss2)) \<tau>\<^sub>1"
-  proof (cases \<F> "GFun f (ss1 @ \<kappa>\<langle>t\<rangle>\<^sub>G # ss2)" \<tau>\<^sub>1 rule: has_type.cases)
+  hence "welltyped \<F> (GFun f (ss1 @ \<kappa>\<langle>t'\<rangle>\<^sub>G # ss2)) \<tau>\<^sub>1"
+  proof (cases \<F> "GFun f (ss1 @ \<kappa>\<langle>t\<rangle>\<^sub>G # ss2)" \<tau>\<^sub>1 rule: welltyped.cases)
     case (GFun \<tau>s)
     show ?thesis
-    proof (rule has_type.GFun)
+    proof (rule welltyped.GFun)
       show "\<F> f = (\<tau>s, \<tau>\<^sub>1)"
         using \<open>\<F> f = (\<tau>s, \<tau>\<^sub>1)\<close> .
     next
-      show "list_all2 (has_type \<F>) (ss1 @ \<kappa>\<langle>t'\<rangle>\<^sub>G # ss2) \<tau>s"
-        using \<open>list_all2 (has_type \<F>) (ss1 @ \<kappa>\<langle>t\<rangle>\<^sub>G # ss2) \<tau>s\<close>
+      show "list_all2 (welltyped \<F>) (ss1 @ \<kappa>\<langle>t'\<rangle>\<^sub>G # ss2) \<tau>s"
+        using \<open>list_all2 (welltyped \<F>) (ss1 @ \<kappa>\<langle>t\<rangle>\<^sub>G # ss2) \<tau>s\<close>
         using GMore.IH
         by (smt (verit, del_insts) list_all2_Cons1 list_all2_append1 list_all2_lengthD)
     qed
